otbn_model/dafny_library/README.md
@@ -1,1 +1,0 @@
-# dafny_library
