otbn_model/libraries/README.md
@@ -1,0 +1,25 @@
+# libraries
+
+Libraries useful for Dafny programs
+
+## Status
+
+At the moment, we're just collecting generally useful Dafny code.
+
+Once we have some amount of code which is used successfully by several projects, we might restructure this repo, informed by the concrete use cases.
+
+So, please do use this library, give feedback, and contribute code, but also expect breaking changes.
+
+## Contributions
+
+Any contributions of generally useful code are welcome, just open a pull request!  Please follow the [library style guidelines](STYLE.md).  If the way to use your new code is not obvious, please add some examples in the `examples` directory to illustrate how to use the code.  We use the [LLVM integrated tester (lit)](https://llvm.org/docs/CommandGuide/lit.html) to test the library files and ensure they all verify correctly.  Please see Dafny's documentation on [installation](https://github.com/dafny-lang/dafny/wiki/INSTALL) and [testing](https://github.com/dafny-lang/dafny/wiki/Running-Dafny's-test-suite) for more details.
+
+## Acknowledgements
+
+Much of this code came from or was inspired by code from the following projects:
+
+* [Ironclad Apps](https://github.com/microsoft/Ironclad/tree/main/ironclad-apps)
+* [IronFleet](https://github.com/microsoft/Ironclad/tree/main/ironfleet)
+* [Vale](https://github.com/project-everest/vale/tree/legacy_dafny)
+* [Verified BetrFS](https://github.com/vmware-labs/verified-betrfs)
+
